compiler/proof_vec/equiv_poly1305_avx.ec
@@ -1,5 +1,61 @@
-require import Int IntDiv CoreMap Jasmin_model.
+require import AllCore IntDiv List CoreMap Jasmin_model.
 require import Poly1305_amd64_5x Poly1305_avx_5x Poly1305_avx_5xp.
+
+hint simplify pow_le0.
+hint simplify powS_minus@1.
+hint simplify
+  (pow2_1, pow2_2, pow2_3, pow2_4, pow2_5, pow2_6, pow2_7, pow2_8)@0.
+
+lemma pow2_32 : 2 ^ 32 = 4294967296.
+proof. by cbv delta. qed.
+
+lemma pow2_64 : 2 ^ 64 = 18446744073709551616.
+proof. by cbv delta. qed.
+
+lemma pow2_128 : 2 ^ 128 = 340282366920938463463374607431768211456.
+proof. by cbv delta. qed.
+
+hint simplify (pow2_32, pow2_64, pow2_128)@0.
+
+axiom W128_unpack_2u64_of_uint i : 
+  unpack_2u64 (W128.of_uint i) = 
+    let i = i %% (2^ W128.size) in
+    (W64.of_uint (i %% 2^64), W64.of_uint (i %/ 2^64)).
+
+hint simplify W128_unpack_2u64_of_uint.
+
+axiom W64_unpack_2u32_of_uint i : 
+  unpack_2u32 (W64.of_uint i) = 
+    let i = i %% (2^ W64.size) in
+    (W32.of_uint (i %% 2^32), W32.of_uint (i %/ 2^32)).
+  
+
+
+hint simplify W64_unpack_2u32_of_uint.
+
+hint simplify (pack_unpack_2u64, unpack_pack_2u64)@0.
+hint simplify (W8.of_uintK, W8.to_uintK')@0.
+hint simplify (W32.of_uintK, W32.to_uintK')@0.
+hint simplify (W64.of_uintK, W64.to_uintK')@0.
+hint simplify (W128.of_uintK, W128.to_uintK')@0.
+
+hint simplify (Array0.get_set_eqE, Array0.get_set_neqE)@0.
+hint simplify (Array1.get_set_eqE, Array1.get_set_neqE)@0.
+hint simplify (Array2.get_set_eqE, Array2.get_set_neqE)@0.
+hint simplify (Array3.get_set_eqE, Array3.get_set_neqE)@0.
+hint simplify (Array4.get_set_eqE, Array4.get_set_neqE)@0.
+hint simplify (Array5.get_set_eqE, Array5.get_set_neqE)@0.
+hint simplify (Array6.get_set_eqE, Array6.get_set_neqE)@0.
+hint simplify (Array7.get_set_eqE, Array7.get_set_neqE)@0.
+hint simplify (Array8.get_set_eqE, Array8.get_set_neqE)@0.
+hint simplify (Array9.get_set_eqE, Array9.get_set_neqE)@0.
+hint simplify (Array10.get_set_eqE, Array10.get_set_neqE)@0.
+
+hint simplify (iota0, iotaS_minus)@0.
+
+(* ------------------------------------------------------------------------------ *)
+(* AVX and its optimized version                                                  *)
+(* ------------------------------------------------------------------------------ *)
 
 equiv poly1305_avx_5x_5xp : 
   Poly1305_avx_5x.M.poly1305 ~ Poly1305_avx_5xp.M.poly1305 :
@@ -15,33 +71,252 @@ proof.
   swap{2} 51 6;sim.
 qed.
 
-op rela5 (x y: (int, W64.t) map) 
-     (xy : (int, W128.t) map) = 
-  xy.[0] = pack_2u64 (y.[0], x.[0]) /\
-  xy.[1] = pack_2u64 (y.[1], x.[1]) /\
-  xy.[2] = pack_2u64 (y.[2], x.[2]) /\
-  xy.[3] = pack_2u64 (y.[3], x.[3]) /\
-  xy.[4] = pack_2u64 (y.[4], x.[4]).
+(* ------------------------------------------------------------------------------ *)
+(* AMD64-5x and AVX-5x                                                            *)
+(* ------------------------------------------------------------------------------ *)
+
+op rela4 (x y: W64.t Array4.t) 
+     (xy : W128.t Array4.t) = 
+  xy.[0] = pack_2u64 (x.[0], y.[0]) /\
+  xy.[1] = pack_2u64 (x.[1], y.[1]) /\
+  xy.[2] = pack_2u64 (x.[2], y.[2]) /\
+  xy.[3] = pack_2u64 (x.[3], y.[3]).
+
+op rela5 (x y: W64.t Array5.t) 
+     (xy : W128.t Array5.t) = 
+  xy.[0] = pack_2u64 (x.[0], y.[0]) /\
+  xy.[1] = pack_2u64 (x.[1], y.[1]) /\
+  xy.[2] = pack_2u64 (x.[2], y.[2]) /\
+  xy.[3] = pack_2u64 (x.[3], y.[3]) /\
+  xy.[4] = pack_2u64 (x.[4], y.[4]).
+
+op is_x5 (z zx5 : W64.t Array5.t) = 
+  zx5.[0] = z.[1] * W64.of_uint 5 /\
+  zx5.[1] = z.[2] * W64.of_uint 5 /\
+  zx5.[2] = z.[3] * W64.of_uint 5 /\
+  zx5.[3] = z.[4] * W64.of_uint 5.
+
+phoare unpack_u26x5x2P x0 y0:
+   [Poly1305_avx_5x.M.unpack_u26x5x2_to_u26x5x2 :
+    s = x0 /\ t = y0 ==> rela5 x0 y0 res] = 1%r.
+proof.
+  proc.
+  (* FIXME "unroll for 3", should work *)
+  unroll 3; rcondt 3; 1: by auto.
+  unroll 7; rcondt 7; 1: by auto.
+  unroll 11; rcondt 11; 1: by auto.
+  unroll 15; rcondt 15; 1: by auto.
+  unroll 19; rcondt 19; 1: by auto.
+  rcondf 23; 1: by auto.
+  wp;skip;cbv delta => />.
+qed.
+
+op bounded_32 (w:W64.t) = W64.to_uint w < 2^32.
+
+op bounded_32_5 (z: W64.t Array5.t) = 
+  bounded_32 z.[0] /\
+  bounded_32 z.[1] /\
+  bounded_32 z.[2] /\
+  bounded_32 z.[3] /\
+  bounded_32 z.[4].
+
+(* axiom to_uint_pos w : 0 <= W64.to_uint w. *)
+axiom to_uint_LAND_r (w1 w2:W64.t) : W64.to_uint (w1 `&` w2) <= W64.to_uint w2.
+
+import StdOrder.IntOrder.
+
+lemma bounded_32_LAND_r (w1 w2:W64.t) : W64.to_uint w2 < 2^32 => bounded_32 (w1 `&` w2).
+proof.
+  rewrite /bounded_32 => h. 
+  apply (ler_lt_trans (to_uint w2)) => //.
+  by apply to_uint_LAND_r.
+qed.
+
+equiv carry_reduceP : Poly1305_amd64_5x.M.carry_reduce ~ Poly1305_avx_5x.M.carry_reduce : 
+        ={x} ==> ={res} /\ bounded_32_5 res{1}.
+proof.
+  proc; wp; skip; rewrite /bounded_32_5 => &m1 &m2 /= -> /=.
+  split; 1: by apply bounded_32_LAND_r; cbv delta.
+  split.
+  + admit.
+  split; 1: by apply bounded_32_LAND_r; cbv delta.
+  split; 1: by apply bounded_32_LAND_r; cbv delta.
+  admit.
+admitted.
+
+equiv clampP : Poly1305_amd64_5x.M.clamp ~ Poly1305_avx_5x.M.clamp : 
+  ={global_mem, k} ==> ={res} /\ bounded_32_5 res{1}.
+proof.
+  proc.
+  seq 2 2 : (={r}); 1: by sim.
+  auto; rewrite /bounded_32_5 /= => ?? -> /=.
+  by rewrite !bounded_32_LAND_r; cbv delta.
+qed.
+  
+axiom pack_mulu_32 w1 w2 : 
+  pack_2u32 (W32.mulu w1 w2) = (zeroext_32_64 w1) * (zeroext_32_64 w2).
+
+hint simplify pack_mulu_32.
+
+axiom zeroext_bounded w : bounded_32 w => zeroext_32_64 (unpack_2u32 w).`1 = w.
+
+lemma zeroext_of_uint i : zeroext_32_64 (W32.of_uint i) = W64.of_uint (i %% W32.modulus).
+proof. by rewrite zeroext_32_64E. qed.
+
+hint simplify zeroext_of_uint.
+
+equiv add_carryP : Poly1305_amd64_5x.M.add_carry ~ Poly1305_avx_5x.M.add_carry : 
+   ={x,y} ==> ={res}.
+proof.
+  proc => /=.
+  conseq (_: Array5.all_eq x{1} x{2}).
+  + move=> ??? ??;apply Array5.ext_eq_all.
+  unroll for {1} 3; unroll for {2} 3.
+  wp; skip; cbv delta => />.
+qed.
+
+equiv hadd_u128P : Poly1305_amd64_5x.M.add_carry ~ Poly1305_avx_5x.M.hadd_u128 :  
+  rela5 x{1} y{1} x{2} ==> ={res}.
+proof.
+  proc *.
+  inline{2} Poly1305_avx_5x.M.hadd_u128; wp.
+  call (add_carryP) => /=.
+  conseq (_: Array5.all_eq x{1} h{2} /\ Array5.all_eq y{1} t{2}).
+  + by move=> ?????;rewrite !Array5.ext_eq_all.
+  unroll for {2} 5; wp; skip => &m1 &m2; cbv delta => [#] 5!-> /=.
+  admit. (* We need to have a symmetry in the code *)
+qed.
+
+hint simplify (VPAND_128_64, VPOR_128_64, VPXOR_128_64)@0.
+
+lemma VPAND_128_64_l w1 w2 : 
+   pack_2u64 w1 `&` w2 = 
+     pack_2u64(w1.`1 `&` (unpack_2u64 w2).`1, w1.`2 `&` (unpack_2u64 w2).`2).
+proof. by rewrite -(pack_unpack_2u64 w2) VPAND_128_64. qed.
+
+hint simplify VPAND_128_64_l@1.
+
+equiv final_mulP : Poly1305_amd64_5x.M.final_mul ~ Poly1305_avx_5x.M.final_mul : 
+  rela5 hx{1} hy{1} hxy{2} /\
+  rela5 s_r2{1} s_r{1} s_r2r{2} /\
+  rela4 s_r2x5{1} s_rx5{1} s_r2rx5{2} ==> ={res}.
+proof.
+  proc => /=.
+  call hadd_u128P => /=.
+  swap{1} 7 3. swap{1} 6 2. swap{1} 6 -1; wp.
+  seq 7 2 : (#post).   
+  + inline *; wp; skip. cbv delta.
+    move=> &m1 &m2 [#] 14!-> />.
+  inline *.
+  wp; skip; cbv delta => &m1 &m2 [#] 5!->; cbv delta.
+  admit. (* again we need condition on size *)
+qed.
+
+equiv remaining_blocksP : Poly1305_amd64_5x.M.remaining_blocks ~ Poly1305_avx_5x.M.remaining_blocks :
+   ={global_mem, in_0} /\ rela5 hx{1} hy{1} hxy{2} /\ 
+            rela5 s_r2{1} s_r2{1} s_r2r2{2} /\ 
+            rela5 s_r4{1} s_r4{1} s_r4r4{2} /\ 
+            rela4 s_r2x5{1} s_r2x5{1} s_r2r2x5{2} /\
+            rela4 s_r4x5{1} s_r4x5{1} s_r4r4x5{2} ==>
+   res{1}.`3 = res{2}.`2 /\
+   rela5 res{1}.`1 res{1}.`2 res{2}.`1.
+proof.
+  proc => /=.
+  swap{1}16 9. swap{1} 15 8; wp.
+  seq 22 9 : (#post). 
+  + admit.
+  inline *.
+  wp; skip; cbv delta => &m1 &m2 [#] 5!->; cbv delta.
+admitted.
+
+equiv first_blockP : Poly1305_amd64_5x.M.first_block ~ Poly1305_avx_5x.M.first_block :
+   ={global_mem, in_0} /\
+   rela5 s_r2{1} s_r2{1} s_r2r2{2} /\
+   rela4 s_r2x5{1} s_r2x5{1} s_r2r2x5{2} ==>
+   res{1}.`3 = res{2}.`2 /\
+   rela5 res{1}.`1 res{1}.`2 res{2}.`1.
+admitted.
+
+axiom W64_leNgt (w1 w2: W64.t) : (w1 `<=` w2) = ! (w2 `<` w1).
 
 equiv poly1305_amd64_avx_5x :
   Poly1305_amd64_5x.M.poly1305 ~ Poly1305_avx_5x.M.poly1305 :
    ={arg} ==> ={res}.
 proof.
   proc=> /=. sim.
-  seq 27 33 : 
-    (#pre /\ ={s_out, s_in, s_inlen, s_k,
-               r, s_r, s_rx5, h, b64, r2, s_r2, s_r2x5} /\ (r=s_r){1}).
-  + seq 21 27 : (#post);last by sim />.
-    while (={i,s_r, r} /\ (r=s_r){1}).
-    + wp;skip => />.
-    
-search "_.[_<-_]".
-    
-
-    admit.
-    sim />.
- sim.
-;1:by sim.
+  seq 20 26 : 
+    (#pre /\ (r=s_r){1} /\ bounded_32_5 r{1} /\
+    ={s_out, s_in, s_inlen, s_k, r, s_r, s_rx5, s_r2x5, h}).
+  + wp. call clampP => /=. 
+    conseq (_ :
+      ={global_mem, out, in_0, inlen, k, s_out, s_in, s_inlen, s_k, s_rx5, s_r2x5, h}) => //.
+    by sim.
+  seq 2 2 : (#pre /\  (is_x5 r s_rx5){1}).
+  + conseq />;unroll for {1} 2; unroll for {2} 2.
+    by wp;skip;cbv delta => />.
+  seq 4 4 : (#pre /\ ={b64}).
+  + by sim />.
   if => //.
-  + sim.
-  seq  
+  seq 0 0 : (#[/:-1]pre); 1: by auto. 
+  seq 5 5 : (#pre /\ ={r2, s_b64, s_r2} /\ (r2 = s_r2){1} /\ bounded_32_5 r2{1}).
+  + conseq |>; wp; call carry_reduceP.
+    by conseq (_: ={r2, s_b64}) => //; sim.
+  seq 2 2 : (#pre /\ (is_x5 r2 s_r2x5){1}).
+  + conseq />;unroll for {1} 2; unroll for {2} 2.
+    by wp;skip;cbv delta => />.
+  seq 0 1 : (#pre); 1: by auto.
+  seq 0 2 : (#pre /\ (r2r = s_r2r){2} /\ rela5 r2{1} r{1} r2r{2}).
+  + wp.
+    exists * r2{2}, r{2}; elim * => r2_R r_R.
+    by call{2} (unpack_u26x5x2P r2_R r_R); skip => />.
+  seq 0 2 : (#pre /\ rela4 s_r2x5{1} s_rx5{1} s_r2rx5{2}).
+  + conseq />;unroll for {2} 2.
+    wp;skip => /> &m2 ????? 4!-> ????? 4!-> ? 4!->.
+    cbv delta.
+    rewrite (zeroext_bounded s_r2{m2}.[1]) // (zeroext_bounded s_r2{m2}.[2]) //.
+    rewrite (zeroext_bounded s_r2{m2}.[3]) // (zeroext_bounded s_r2{m2}.[4]) //.
+    rewrite (zeroext_bounded s_r{m2}.[1]) // (zeroext_bounded s_r{m2}.[2]) //.
+    by rewrite (zeroext_bounded s_r{m2}.[3]) // (zeroext_bounded s_r{m2}.[4]).
+  seq 0 2 : (#pre /\ (r2r2 = s_r2r2){2} /\ rela5 r2{1} r2{1} r2r2{2}).
+  + wp; conseq />.
+    exists * r2{2}; elim * => r2_R.
+    by call{2} (unpack_u26x5x2P r2_R r2_R); skip => />.
+  seq 0 2 : (#pre /\ rela4 s_r2x5{1} s_r2x5{1} s_r2r2x5{2}).
+  + conseq />;unroll for {2} 2.
+    wp;skip => /> &m2 ????? 4!-> ????? 4!-> ????? ???? ? 4!->.
+    cbv delta.
+    rewrite (zeroext_bounded s_r2{m2}.[1]) // (zeroext_bounded s_r2{m2}.[2]) //.
+    by rewrite (zeroext_bounded s_r2{m2}.[3]) // (zeroext_bounded s_r2{m2}.[4]).
+  seq 1 1 : (#pre /\ (b64 = s_b64){1}); 1: by auto. 
+  if => //.
+  + seq 4 3 : (#pre /\ ={r4} /\ (r4 = s_r4){1} /\ bounded_32_5 r4{1}).
+      + conseq |>; wp;call carry_reduceP.
+        by conseq (_: ={r4}) => //; sim.
+      seq 0 2 : (#pre /\ (r4r4=s_r4r4){2} /\ rela5 r4{1} r4{1} r4r4{2}).
+      + wp; exists * r4{2}; elim * => r4_R.
+      by call{2} (unpack_u26x5x2P r4_R r4_R); skip => />.
+    seq 2 2 : (#pre /\ rela4 s_r4x5{1} s_r4x5{1} s_r4r4x5{2}).
+    + unroll for {1} 2. unroll for {2} 2.
+      wp; skip => /> &m1 &m2 ????? ???? ????? ???? ????? ???? ????? ???? ? ????? ? 4!->.
+      cbv delta.
+      rewrite (zeroext_bounded s_r4{m1}.[1]) // (zeroext_bounded s_r4{m1}.[2]) //.
+      by rewrite (zeroext_bounded s_r4{m1}.[3]) // (zeroext_bounded s_r4{m1}.[4]).
+    call final_mulP; conseq (_ : rela5 hx{1} hy{1} hxy{2} /\ ={in_0}) => //.
+    while (={global_mem, b64, in_0} /\ 
+            rela5 hx{1} hy{1} hxy{2} /\ 
+            rela5 s_r2{1} s_r2{1} s_r2r2{2} /\ 
+            rela5 s_r4{1} s_r4{1} s_r4r4{2} /\ 
+            rela4 s_r2x5{1} s_r2x5{1} s_r2r2x5{2} /\
+            rela4 s_r4x5{1} s_r4x5{1} s_r4r4x5{2}).
+    + by wp; call remaining_blocksP; wp; skip.
+    by wp; call first_blockP; wp; skip.  
+  rcondf{1} 5.  
+  + move=> &m2; wp; conseq (_: true) => //.
+    move=> |> ????????. admit. (* would be simpler if we use unsigned comparison *)
+  rcondf{2} 5.
+  + move=> &m1; wp; conseq (_: true) => //.
+    move=> |> ????????.  admit. (* would be simpler if we use unsigned comparison *) 
+  call final_mulP; conseq (_ : rela5 hx{1} hy{1} hxy{2} /\ ={in_0}) => //.
+  by wp; call first_blockP; wp; skip.  
+qed.
+
