compiler/proof_vec/poly1305_avx_5xp_ct.ec
@@ -1,5 +1,6 @@
 require import List Jasmin_model Int IntDiv CoreMap.
 
+
 abbrev zero_u128 = W128.of_uint 0.
 
 
@@ -15,7 +16,7 @@ abbrev mask26_u128 = W128.of_uint 1237940020838636201256681471.
 module M = {
   var leakages : leakages_t
   
-  proc add (x:(int,W64.t)map, y:(int,W64.t)map) : (int,W64.t)map = {
+  proc add (x:W64.t Array5.t, y:W64.t Array5.t) : W64.t Array5.t = {
     var i:int;
     
     leakages <- LeakFor(0,5) :: LeakExpr([]) :: leakages;
@@ -28,7 +29,7 @@ module M = {
     return (x);
   }
   
-  proc add_carry (x:(int,W64.t)map, y:(int,W64.t)map) : (int,W64.t)map = {
+  proc add_carry (x:W64.t Array5.t, y:W64.t Array5.t) : W64.t Array5.t = {
     var i:int;
     var c:W64.t;
     
@@ -52,7 +53,7 @@ module M = {
     return (x);
   }
   
-  proc add_u128 (x:(int,W128.t)map, y:(int,W128.t)map) : (int,W128.t)map = {
+  proc add_u128 (x:W128.t Array5.t, y:W128.t Array5.t) : W128.t Array5.t = {
     var i:int;
     
     leakages <- LeakFor(0,5) :: LeakExpr([]) :: leakages;
@@ -65,12 +66,12 @@ module M = {
     return (x);
   }
   
-  proc hadd_u128 (x:(int,W128.t)map) : (int,W64.t)map = {
-    var h:(int,W64.t)map;
+  proc hadd_u128 (x:W128.t Array5.t) : W64.t Array5.t = {
+    var h:W64.t Array5.t;
     var i:int;
-    var t:(int,W64.t)map;
-    h <- (array_init_64 5);
-    t <- (array_init_64 5);
+    var t:W64.t Array5.t;
+    h <- Array5.init;
+    t <- Array5.init;
     leakages <- LeakFor(0,5) :: LeakExpr([]) :: leakages;
     i <- 0;
     while (i < 5) {
@@ -85,20 +86,14 @@ module M = {
     return (h);
   }
   
-  proc freeze (x:(int,W64.t)map) : (int,W64.t)map = {
-    var i:int;
-    var ox:(int,W64.t)map;
-    var mp:(int,W64.t)map;
+  proc freeze (x:W64.t Array5.t) : W64.t Array5.t = {
+    var ox:W64.t Array5.t;
+    var mp:W64.t Array5.t;
     var n:W64.t;
-    mp <- (array_init_64 5);
-    ox <- (array_init_64 5);
-    leakages <- LeakFor(0,5) :: LeakExpr([]) :: leakages;
-    i <- 0;
-    while (i < 5) {
-      leakages <- LeakExpr([]) :: leakages;
-      ox.[i] <- x.[i];
-      i <- i + 1;
-    }
+    mp <- Array5.init;
+    ox <- Array5.init;
+    leakages <- LeakExpr([]) :: leakages;
+    ox <- x;
     leakages <- LeakExpr([]) :: leakages;
     mp.[0] <- (W64.of_uint 5);
     leakages <- LeakExpr([]) :: leakages;
@@ -152,12 +147,12 @@ module M = {
     return (x);
   }
   
-  proc unpack (global_mem : global_mem_t, m:W64.t) : (int,W64.t)map = {
-    var x:(int,W64.t)map;
+  proc unpack (global_mem : global_mem_t, m:W64.t) : W64.t Array5.t = {
+    var x:W64.t Array5.t;
     var m0:W64.t;
     var m1:W64.t;
     var t:W64.t;
-    x <- (array_init_64 5);
+    x <- Array5.init;
     leakages <- LeakExpr([(m + (W64.of_uint (8 * 0)))]) :: leakages;
     m0 <- (loadW64 global_mem (m + (W64.of_uint (8 * 0))));
     leakages <- LeakExpr([(m + (W64.of_uint (8 * 1)))]) :: leakages;
@@ -197,12 +192,12 @@ module M = {
     return (x);
   }
   
-  proc mulmod_12 (x:(int,W64.t)map, y:(int,W64.t)map, yx5:(int,W64.t)map) : 
-  (int,W64.t)map = {
-    var t:(int,W64.t)map;
-    var z:(int,W64.t)map;
-    t <- (array_init_64 5);
-    z <- (array_init_64 3);
+  proc mulmod_12 (x:W64.t Array5.t, y:W64.t Array5.t, yx5:W64.t Array4.t) : 
+  W64.t Array5.t = {
+    var t:W64.t Array5.t;
+    var z:W64.t Array3.t;
+    t <- Array5.init;
+    z <- Array3.init;
     leakages <- LeakExpr([]) :: leakages;
     t.[0] <- x.[0];
     leakages <- LeakExpr([]) :: leakages;
@@ -356,9 +351,9 @@ module M = {
     return (x);
   }
   
-  proc carry_reduce (x:(int,W64.t)map) : (int,W64.t)map = {
-    var z:(int,W64.t)map;
-    z <- (array_init_64 2);
+  proc carry_reduce (x:W64.t Array5.t) : W64.t Array5.t = {
+    var z:W64.t Array2.t;
+    z <- Array2.init;
     leakages <- LeakExpr([]) :: leakages;
     z.[0] <- x.[0];
     leakages <- LeakExpr([]) :: leakages;
@@ -420,11 +415,11 @@ module M = {
     return (x);
   }
   
-  proc unpack_u26x5x2_to_u26x5x2 (s:(int,W64.t)map, t:(int,W64.t)map) : 
-  (int,W128.t)map = {
-    var r:(int,W128.t)map;
+  proc unpack_u26x5x2_to_u26x5x2 (s:W64.t Array5.t, t:W64.t Array5.t) : 
+  W128.t Array5.t = {
+    var r:W128.t Array5.t;
     var i:int;
-    r <- (array_init_128 5);
+    r <- Array5.init;
     leakages <- LeakFor(0,5) :: LeakExpr([]) :: leakages;
     i <- 0;
     while (i < 5) {
@@ -440,14 +435,14 @@ module M = {
   }
   
   proc unpack_u128x2_to_u26x5x2 (global_mem : global_mem_t, m:W64.t) : 
-  (int,W128.t)map = {
-    var r:(int,W128.t)map;
+  W128.t Array5.t = {
+    var r:W128.t Array5.t;
     var s128:W128.t;
     var t128:W128.t;
     var t1:W128.t;
     var t2:W128.t;
     var t3:W128.t;
-    r <- (array_init_128 5);
+    r <- Array5.init;
     leakages <- LeakExpr([(m + (W64.of_uint (8 * 0)))]) :: leakages;
     s128 <- x86_MOVD_64 (loadW64 global_mem (m + (W64.of_uint (8 * 0))));
     leakages <- LeakExpr([(m + (W64.of_uint (8 * 2)))]) :: leakages;
@@ -485,12 +480,12 @@ module M = {
     return (r);
   }
   
-  proc mulmod_u128 (x:(int,W128.t)map, y:(int,W128.t)map, yx5:(int,W128.t)map) : 
-  (int,W128.t)map = {
-    var t:(int,W128.t)map;
-    var z:(int,W128.t)map;
-    t <- (array_init_128 5);
-    z <- (array_init_128 5);
+  proc mulmod_u128 (x:W128.t Array5.t, y:W128.t Array5.t, yx5:W128.t Array4.t) : 
+  W128.t Array5.t = {
+    var t:W128.t Array5.t;
+    var z:W128.t Array5.t;
+    t <- Array5.init;
+    z <- Array5.init;
     leakages <- LeakExpr([]) :: leakages;
     t.[0] <- x86_VPMULU_128 x.[0] y.[0];
     leakages <- LeakExpr([]) :: leakages;
@@ -587,16 +582,16 @@ module M = {
   }
   
   proc mulmod_u128_prefetch (global_mem : global_mem_t, in_0:W64.t,
-                                                        x:(int,W128.t)map,
-                                                        y:(int,W128.t)map,
-                                                        yx5:(int,W128.t)map) : 
-  (int,W128.t)map * (int,W128.t)map = {
-    var xy0:(int,W128.t)map;
-    var t:(int,W128.t)map;
-    var z:(int,W128.t)map;
-    t <- (array_init_128 5);
-    xy0 <- (array_init_128 5);
-    z <- (array_init_128 5);
+                                                        x:W128.t Array5.t,
+                                                        y:W128.t Array5.t,
+                                                        yx5:W128.t Array4.t) : 
+  W128.t Array5.t * W128.t Array5.t = {
+    var xy0:W128.t Array5.t;
+    var t:W128.t Array5.t;
+    var z:W128.t Array5.t;
+    t <- Array5.init;
+    xy0 <- Array5.init;
+    z <- Array5.init;
     leakages <- LeakExpr([]) :: leakages;
     t.[0] <- x86_VPMULU_128 x.[0] y.[0];
     leakages <- LeakExpr([]) :: leakages;
@@ -695,17 +690,17 @@ module M = {
   }
   
   proc mulmod_add_u128_prefetch (global_mem : global_mem_t, in_0:W64.t,
-                                                            u:(int,W128.t)map,
-                                                            x:(int,W128.t)map,
-                                                            y:(int,W128.t)map,
-                                                            yx5:(int,W128.t)map) : 
-  (int,W128.t)map * (int,W128.t)map = {
-    var xy1:(int,W128.t)map;
-    var t:(int,W128.t)map;
-    var z:(int,W128.t)map;
-    t <- (array_init_128 5);
-    xy1 <- (array_init_128 5);
-    z <- (array_init_128 5);
+                                                            u:W128.t Array5.t,
+                                                            x:W128.t Array5.t,
+                                                            y:W128.t Array5.t,
+                                                            yx5:W128.t Array4.t) : 
+  W128.t Array5.t * W128.t Array5.t = {
+    var xy1:W128.t Array5.t;
+    var t:W128.t Array5.t;
+    var z:W128.t Array5.t;
+    t <- Array5.init;
+    xy1 <- Array5.init;
+    z <- Array5.init;
     leakages <- LeakExpr([]) :: leakages;
     t.[0] <- x86_VPMULU_128 x.[0] y.[0];
     leakages <- LeakExpr([]) :: leakages;
@@ -805,9 +800,9 @@ module M = {
     return (u, xy1);
   }
   
-  proc carry_reduce_u128 (x:(int,W128.t)map) : (int,W128.t)map = {
-    var z:(int,W128.t)map;
-    z <- (array_init_128 2);
+  proc carry_reduce_u128 (x:W128.t Array5.t) : W128.t Array5.t = {
+    var z:W128.t Array2.t;
+    z <- Array2.init;
     leakages <- LeakExpr([]) :: leakages;
     z.[0] <- x86_VPSRL_2u64 x.[0] (W8.of_uint 26);
     leakages <- LeakExpr([]) :: leakages;
@@ -855,9 +850,9 @@ module M = {
     return (x);
   }
   
-  proc clamp (global_mem : global_mem_t, k:W64.t) : (int,W64.t)map = {
-    var r:(int,W64.t)map;
-    r <- (array_init_64 5);
+  proc clamp (global_mem : global_mem_t, k:W64.t) : W64.t Array5.t = {
+    var r:W64.t Array5.t;
+    r <- Array5.init;
     leakages <- LeakExpr([]) :: leakages;
     r <@ unpack (global_mem, k);
     leakages <- LeakExpr([]) :: leakages;
@@ -873,9 +868,9 @@ module M = {
     return (r);
   }
   
-  proc load (global_mem : global_mem_t, in_0:W64.t) : (int,W64.t)map = {
-    var x:(int,W64.t)map;
-    x <- (array_init_64 5);
+  proc load (global_mem : global_mem_t, in_0:W64.t) : W64.t Array5.t = {
+    var x:W64.t Array5.t;
+    x <- Array5.init;
     leakages <- LeakExpr([]) :: leakages;
     x <@ unpack (global_mem, in_0);
     leakages <- LeakExpr([]) :: leakages;
@@ -884,15 +879,15 @@ module M = {
   }
   
   proc load_last (global_mem : global_mem_t, in_0:W64.t, inlen:W64.t) : 
-  (int,W64.t)map = {
-    var x:(int,W64.t)map;
+  W64.t Array5.t = {
+    var x:W64.t Array5.t;
     var i:int;
-    var m:(int,W64.t)map;
+    var m:W64.t Array2.t;
     var c:W64.t;
     var n:W64.t;
     var t:W64.t;
-    m <- (array_init_64 2);
-    x <- (array_init_64 5);
+    m <- Array2.init;
+    x <- Array5.init;
     leakages <- LeakFor(0,2) :: LeakExpr([]) :: leakages;
     i <- 0;
     while (i < 2) {
@@ -900,16 +895,16 @@ module M = {
       m.[i] <- (W64.of_uint 0);
       i <- i + 1;
     }
-    leakages <- LeakCond((inlen `<` (W64.of_uint 8))) :: LeakExpr([]) :: leakages;
-    if ((inlen `<` (W64.of_uint 8))) {
+    leakages <- LeakCond((inlen \ult (W64.of_uint 8))) :: LeakExpr([]) :: leakages;
+    if ((inlen \ult (W64.of_uint 8))) {
       leakages <- LeakExpr([]) :: leakages;
       c <- (W64.of_uint 0);
       leakages <- LeakExpr([]) :: leakages;
       n <- (W64.of_uint 0);
       
-      leakages <- LeakCond((c `<` inlen)) :: LeakExpr([]) :: leakages;
+      leakages <- LeakCond((c \ult inlen)) :: LeakExpr([]) :: leakages;
       
-      while ((c `<` inlen)) {
+      while ((c \ult inlen)) {
         leakages <- LeakExpr([(in_0 + c)]) :: leakages;
         t <- (zeroext_8_64 (loadW8 global_mem (in_0 + c)));
         leakages <- LeakExpr([]) :: leakages;
@@ -920,7 +915,7 @@ module M = {
         n <- (n + (W64.of_uint 8));
         leakages <- LeakExpr([]) :: leakages;
         c <- (c + (W64.of_uint 1));
-      leakages <- LeakCond((c `<` inlen)) :: LeakExpr([]) :: leakages;
+      leakages <- LeakCond((c \ult inlen)) :: LeakExpr([]) :: leakages;
       
       }
       leakages <- LeakExpr([]) :: leakages;
@@ -941,9 +936,9 @@ module M = {
       leakages <- LeakExpr([]) :: leakages;
       n <- (W64.of_uint 0);
       
-      leakages <- LeakCond((c `<` inlen)) :: LeakExpr([]) :: leakages;
+      leakages <- LeakCond((c \ult inlen)) :: LeakExpr([]) :: leakages;
       
-      while ((c `<` inlen)) {
+      while ((c \ult inlen)) {
         leakages <- LeakExpr([(in_0 + c)]) :: leakages;
         t <- (zeroext_8_64 (loadW8 global_mem (in_0 + c)));
         leakages <- LeakExpr([]) :: leakages;
@@ -954,7 +949,7 @@ module M = {
         n <- (n + (W64.of_uint 8));
         leakages <- LeakExpr([]) :: leakages;
         c <- (c + (W64.of_uint 1));
-      leakages <- LeakCond((c `<` inlen)) :: LeakExpr([]) :: leakages;
+      leakages <- LeakCond((c \ult inlen)) :: LeakExpr([]) :: leakages;
       
       }
       leakages <- LeakExpr([]) :: leakages;
@@ -999,7 +994,7 @@ module M = {
     return (x);
   }
   
-  proc pack (global_mem : global_mem_t, y:W64.t, x:(int,W64.t)map) : 
+  proc pack (global_mem : global_mem_t, y:W64.t, x:W64.t Array5.t) : 
   global_mem_t = {
     var t:W64.t;
     var t1:W64.t;
@@ -1044,15 +1039,15 @@ module M = {
   }
   
   proc first_block (global_mem : global_mem_t, in_0:W64.t,
-                                               s_r2r2:(int,W128.t)map,
-                                               s_r2r2x5:(int,W128.t)map) : 
-  (int,W128.t)map * W64.t = {
-    var hxy:(int,W128.t)map;
-    var xy0:(int,W128.t)map;
-    var xy1:(int,W128.t)map;
-    hxy <- (array_init_128 5);
-    xy0 <- (array_init_128 5);
-    xy1 <- (array_init_128 5);
+                                               s_r2r2:W128.t Array5.t,
+                                               s_r2r2x5:W128.t Array4.t) : 
+  W128.t Array5.t * W64.t = {
+    var hxy:W128.t Array5.t;
+    var xy0:W128.t Array5.t;
+    var xy1:W128.t Array5.t;
+    hxy <- Array5.init;
+    xy0 <- Array5.init;
+    xy1 <- Array5.init;
     leakages <- LeakExpr([]) :: leakages;
     xy0 <@ unpack_u128x2_to_u26x5x2 (global_mem, in_0);
     leakages <- LeakExpr([]) :: leakages;
@@ -1070,17 +1065,17 @@ module M = {
     return (hxy, in_0);
   }
   
-  proc remaining_blocks (global_mem : global_mem_t, hxy:(int,W128.t)map,
+  proc remaining_blocks (global_mem : global_mem_t, hxy:W128.t Array5.t,
                                                     in_0:W64.t,
-                                                    s_r4r4:(int,W128.t)map,
-                                                    s_r4r4x5:(int,W128.t)map,
-                                                    s_r2r2:(int,W128.t)map,
-                                                    s_r2r2x5:(int,W128.t)map) : 
-  (int,W128.t)map * W64.t = {
-    var xy0:(int,W128.t)map;
-    var xy1:(int,W128.t)map;
-    xy0 <- (array_init_128 5);
-    xy1 <- (array_init_128 5);
+                                                    s_r4r4:W128.t Array5.t,
+                                                    s_r4r4x5:W128.t Array4.t,
+                                                    s_r2r2:W128.t Array5.t,
+                                                    s_r2r2x5:W128.t Array4.t) : 
+  W128.t Array5.t * W64.t = {
+    var xy0:W128.t Array5.t;
+    var xy1:W128.t Array5.t;
+    xy0 <- Array5.init;
+    xy1 <- Array5.init;
     leakages <- LeakExpr([]) :: leakages;
     (hxy, xy0) <@ mulmod_u128_prefetch (global_mem, in_0, hxy, s_r4r4,
     s_r4r4x5);
@@ -1098,10 +1093,10 @@ module M = {
     return (hxy, in_0);
   }
   
-  proc final_mul (hxy:(int,W128.t)map, s_r2r:(int,W128.t)map,
-                  s_r2rx5:(int,W128.t)map) : (int,W64.t)map = {
-    var h:(int,W64.t)map;
-    h <- (array_init_64 5);
+  proc final_mul (hxy:W128.t Array5.t, s_r2r:W128.t Array5.t,
+                  s_r2rx5:W128.t Array4.t) : W64.t Array5.t = {
+    var h:W64.t Array5.t;
+    h <- Array5.init;
     leakages <- LeakExpr([]) :: leakages;
     hxy <@ mulmod_u128 (hxy, s_r2r, s_r2rx5);
     leakages <- LeakExpr([]) :: leakages;
@@ -1117,56 +1112,52 @@ module M = {
     var s_in:W64.t;
     var s_inlen:W64.t;
     var s_k:W64.t;
-    var r:(int,W64.t)map;
+    var r:W64.t Array5.t;
+    var s_r:W64.t Array5.t;
     var i:int;
-    var s_r:(int,W64.t)map;
-    var i_0:int;
     var t:W64.t;
-    var s_rx5:(int,W64.t)map;
-    var h:(int,W64.t)map;
+    var s_rx5:W64.t Array4.t;
+    var h:W64.t Array5.t;
     var b64:W64.t;
     var s_b64:W64.t;
-    var i_1:int;
-    var r2:(int,W64.t)map;
-    var i_2:int;
-    var s_r2:(int,W64.t)map;
-    var s_r2x5:(int,W64.t)map;
-    var r2r:(int,W128.t)map;
-    var s_r2r:(int,W128.t)map;
+    var r2:W64.t Array5.t;
+    var s_r2:W64.t Array5.t;
+    var s_r2x5:W64.t Array4.t;
+    var r2r:W128.t Array5.t;
+    var s_r2r:W128.t Array5.t;
     var t_u128:W128.t;
-    var s_r2rx5:(int,W128.t)map;
-    var r2r2:(int,W128.t)map;
-    var s_r2r2:(int,W128.t)map;
-    var s_r2r2x5:(int,W128.t)map;
-    var i_3:int;
-    var r4:(int,W64.t)map;
-    var r4r4:(int,W128.t)map;
-    var s_r4r4:(int,W128.t)map;
-    var s_r4r4x5:(int,W128.t)map;
-    var hxy:(int,W128.t)map;
+    var s_r2rx5:W128.t Array4.t;
+    var r2r2:W128.t Array5.t;
+    var s_r2r2:W128.t Array5.t;
+    var s_r2r2x5:W128.t Array4.t;
+    var r4:W64.t Array5.t;
+    var r4r4:W128.t Array5.t;
+    var s_r4r4:W128.t Array5.t;
+    var s_r4r4x5:W128.t Array4.t;
+    var hxy:W128.t Array5.t;
     var b16:W64.t;
-    var x:(int,W64.t)map;
-    var s:(int,W64.t)map;
-    h <- (array_init_64 5);
-    hxy <- (array_init_128 5);
-    r <- (array_init_64 5);
-    r2 <- (array_init_64 5);
-    r2r <- (array_init_128 5);
-    r2r2 <- (array_init_128 5);
-    r4 <- (array_init_64 5);
-    r4r4 <- (array_init_128 5);
-    s <- (array_init_64 5);
-    s_r <- (array_init_64 5);
-    s_r2 <- (array_init_64 5);
-    s_r2r <- (array_init_128 5);
-    s_r2r2 <- (array_init_128 5);
-    s_r2r2x5 <- (array_init_128 4);
-    s_r2rx5 <- (array_init_128 4);
-    s_r2x5 <- (array_init_64 4);
-    s_r4r4 <- (array_init_128 5);
-    s_r4r4x5 <- (array_init_128 4);
-    s_rx5 <- (array_init_64 4);
-    x <- (array_init_64 5);
+    var x:W64.t Array5.t;
+    var s:W64.t Array5.t;
+    h <- Array5.init;
+    hxy <- Array5.init;
+    r <- Array5.init;
+    r2 <- Array5.init;
+    r2r <- Array5.init;
+    r2r2 <- Array5.init;
+    r4 <- Array5.init;
+    r4r4 <- Array5.init;
+    s <- Array5.init;
+    s_r <- Array5.init;
+    s_r2 <- Array5.init;
+    s_r2r <- Array5.init;
+    s_r2r2 <- Array5.init;
+    s_r2r2x5 <- Array4.init;
+    s_r2rx5 <- Array4.init;
+    s_r2x5 <- Array4.init;
+    s_r4r4 <- Array5.init;
+    s_r4r4x5 <- Array4.init;
+    s_rx5 <- Array4.init;
+    x <- Array5.init;
     leakages <- LeakExpr([]) :: leakages;
     s_out <- out;
     leakages <- LeakExpr([]) :: leakages;
@@ -1177,139 +1168,99 @@ module M = {
     s_k <- k;
     leakages <- LeakExpr([]) :: leakages;
     r <@ clamp (global_mem, k);
+    leakages <- LeakExpr([]) :: leakages;
+    s_r <- r;
+    leakages <- LeakFor(0,4) :: LeakExpr([]) :: leakages;
+    i <- 0;
+    while (i < 4) {
+      leakages <- LeakExpr([]) :: leakages;
+      t <- (r.[(i + 1)] * (W64.of_uint 5));
+      leakages <- LeakExpr([]) :: leakages;
+      s_rx5.[i] <- t;
+      i <- i + 1;
+    }
     leakages <- LeakFor(0,5) :: LeakExpr([]) :: leakages;
     i <- 0;
     while (i < 5) {
       leakages <- LeakExpr([]) :: leakages;
-      s_r.[i] <- r.[i];
+      h.[i] <- (W64.of_uint 0);
       i <- i + 1;
-    }
-    leakages <- LeakFor(0,4) :: LeakExpr([]) :: leakages;
-    i_0 <- 0;
-    while (i_0 < 4) {
-      leakages <- LeakExpr([]) :: leakages;
-      t <- (r.[(i_0 + 1)] * (W64.of_uint 5));
-      leakages <- LeakExpr([]) :: leakages;
-      s_rx5.[i_0] <- t;
-      i_0 <- i_0 + 1;
-    }
-    leakages <- LeakFor(0,5) :: LeakExpr([]) :: leakages;
-    i_0 <- 0;
-    while (i_0 < 5) {
-      leakages <- LeakExpr([]) :: leakages;
-      h.[i_0] <- (W64.of_uint 0);
-      i_0 <- i_0 + 1;
     }
     leakages <- LeakExpr([]) :: leakages;
     b64 <- inlen;
     leakages <- LeakExpr([]) :: leakages;
     b64 <- (b64 `>>` (W8.of_uint 6));
-    leakages <- LeakCond(((W64.of_uint 0) `<` b64)) :: LeakExpr([]) :: leakages;
-    if (((W64.of_uint 0) `<` b64)) {
+    leakages <- LeakCond(((W64.of_uint 0) \ult b64)) :: LeakExpr([]) :: leakages;
+    if (((W64.of_uint 0) \ult b64)) {
       leakages <- LeakExpr([]) :: leakages;
       s_b64 <- b64;
-      leakages <- LeakFor(0,5) :: LeakExpr([]) :: leakages;
-      i_1 <- 0;
-      while (i_1 < 5) {
-        leakages <- LeakExpr([]) :: leakages;
-        r2.[i_1] <- r.[i_1];
-        i_1 <- i_1 + 1;
-      }
+      leakages <- LeakExpr([]) :: leakages;
+      r2 <- r;
       leakages <- LeakExpr([]) :: leakages;
       r2 <@ mulmod_12 (r2, s_r, s_rx5);
       leakages <- LeakExpr([]) :: leakages;
       r2 <@ carry_reduce (r2);
-      leakages <- LeakFor(0,5) :: LeakExpr([]) :: leakages;
-      i_2 <- 0;
-      while (i_2 < 5) {
-        leakages <- LeakExpr([]) :: leakages;
-        s_r2.[i_2] <- r2.[i_2];
-        i_2 <- i_2 + 1;
-      }
+      leakages <- LeakExpr([]) :: leakages;
+      s_r2 <- r2;
       leakages <- LeakFor(0,4) :: LeakExpr([]) :: leakages;
-      i_0 <- 0;
-      while (i_0 < 4) {
+      i <- 0;
+      while (i < 4) {
         leakages <- LeakExpr([]) :: leakages;
-        t <- (r2.[(i_0 + 1)] * (W64.of_uint 5));
+        t <- (r2.[(i + 1)] * (W64.of_uint 5));
         leakages <- LeakExpr([]) :: leakages;
-        s_r2x5.[i_0] <- t;
-        i_0 <- i_0 + 1;
-      }
-      leakages <- LeakFor(0,5) :: LeakExpr([]) :: leakages;
-      i_0 <- 0;
-      while (i_0 < 5) {
-        leakages <- LeakExpr([]) :: leakages;
-        r.[i_0] <- s_r.[i_0];
-        i_0 <- i_0 + 1;
+        s_r2x5.[i] <- t;
+        i <- i + 1;
       }
       leakages <- LeakExpr([]) :: leakages;
+      r <- s_r;
+      leakages <- LeakExpr([]) :: leakages;
       r2r <@ unpack_u26x5x2_to_u26x5x2 (r2, r);
-      leakages <- LeakFor(0,5) :: LeakExpr([]) :: leakages;
-      i_0 <- 0;
-      while (i_0 < 5) {
-        leakages <- LeakExpr([]) :: leakages;
-        s_r2r.[i_0] <- r2r.[i_0];
-        i_0 <- i_0 + 1;
-      }
+      leakages <- LeakExpr([]) :: leakages;
+      s_r2r <- r2r;
       leakages <- LeakFor(0,4) :: LeakExpr([]) :: leakages;
-      i_0 <- 0;
-      while (i_0 < 4) {
+      i <- 0;
+      while (i < 4) {
         leakages <- LeakExpr([]) :: leakages;
-        t_u128 <- x86_VPMULU_128 r2r.[(i_0 + 1)] five_u128;
+        t_u128 <- x86_VPMULU_128 r2r.[(i + 1)] five_u128;
         leakages <- LeakExpr([]) :: leakages;
-        s_r2rx5.[i_0] <- t_u128;
-        i_0 <- i_0 + 1;
+        s_r2rx5.[i] <- t_u128;
+        i <- i + 1;
       }
       leakages <- LeakExpr([]) :: leakages;
       r2r2 <@ unpack_u26x5x2_to_u26x5x2 (r2, r2);
-      leakages <- LeakFor(0,5) :: LeakExpr([]) :: leakages;
-      i_0 <- 0;
-      while (i_0 < 5) {
-        leakages <- LeakExpr([]) :: leakages;
-        s_r2r2.[i_0] <- r2r2.[i_0];
-        i_0 <- i_0 + 1;
-      }
+      leakages <- LeakExpr([]) :: leakages;
+      s_r2r2 <- r2r2;
       leakages <- LeakFor(0,4) :: LeakExpr([]) :: leakages;
-      i_0 <- 0;
-      while (i_0 < 4) {
+      i <- 0;
+      while (i < 4) {
         leakages <- LeakExpr([]) :: leakages;
-        t_u128 <- x86_VPMULU_128 r2r2.[(i_0 + 1)] five_u128;
+        t_u128 <- x86_VPMULU_128 r2r2.[(i + 1)] five_u128;
         leakages <- LeakExpr([]) :: leakages;
-        s_r2r2x5.[i_0] <- t_u128;
-        i_0 <- i_0 + 1;
+        s_r2r2x5.[i] <- t_u128;
+        i <- i + 1;
       }
       leakages <- LeakExpr([]) :: leakages;
       b64 <- s_b64;
-      leakages <- LeakCond(((W64.of_uint 1) `<` b64)) :: LeakExpr([]) :: leakages;
-      if (((W64.of_uint 1) `<` b64)) {
-        leakages <- LeakFor(0,5) :: LeakExpr([]) :: leakages;
-        i_3 <- 0;
-        while (i_3 < 5) {
-          leakages <- LeakExpr([]) :: leakages;
-          r4.[i_3] <- r2.[i_3];
-          i_3 <- i_3 + 1;
-        }
+      leakages <- LeakCond(((W64.of_uint 1) \ult b64)) :: LeakExpr([]) :: leakages;
+      if (((W64.of_uint 1) \ult b64)) {
+        leakages <- LeakExpr([]) :: leakages;
+        r4 <- r2;
         leakages <- LeakExpr([]) :: leakages;
         r4 <@ mulmod_12 (r4, s_r2, s_r2x5);
         leakages <- LeakExpr([]) :: leakages;
         r4 <@ carry_reduce (r4);
         leakages <- LeakExpr([]) :: leakages;
         r4r4 <@ unpack_u26x5x2_to_u26x5x2 (r4, r4);
-        leakages <- LeakFor(0,5) :: LeakExpr([]) :: leakages;
-        i_0 <- 0;
-        while (i_0 < 5) {
-          leakages <- LeakExpr([]) :: leakages;
-          s_r4r4.[i_0] <- r4r4.[i_0];
-          i_0 <- i_0 + 1;
-        }
+        leakages <- LeakExpr([]) :: leakages;
+        s_r4r4 <- r4r4;
         leakages <- LeakFor(0,4) :: LeakExpr([]) :: leakages;
-        i_0 <- 0;
-        while (i_0 < 4) {
+        i <- 0;
+        while (i < 4) {
           leakages <- LeakExpr([]) :: leakages;
-          t_u128 <- x86_VPMULU_128 r4r4.[(i_0 + 1)] five_u128;
+          t_u128 <- x86_VPMULU_128 r4r4.[(i + 1)] five_u128;
           leakages <- LeakExpr([]) :: leakages;
-          s_r4r4x5.[i_0] <- t_u128;
-          i_0 <- i_0 + 1;
+          s_r4r4x5.[i] <- t_u128;
+          i <- i + 1;
         }
       } else {
         
@@ -1323,9 +1274,9 @@ module M = {
       leakages <- LeakExpr([]) :: leakages;
       b64 <- (b64 - (W64.of_uint 1));
       
-      leakages <- LeakCond(((W64.of_uint 0) `<` b64)) :: LeakExpr([]) :: leakages;
+      leakages <- LeakCond(((W64.of_uint 0) \ult b64)) :: LeakExpr([]) :: leakages;
       
-      while (((W64.of_uint 0) `<` b64)) {
+      while (((W64.of_uint 0) \ult b64)) {
         leakages <- LeakExpr([]) :: leakages;
         b64 <- (b64 - (W64.of_uint 1));
         leakages <- LeakExpr([]) :: leakages;
@@ -1335,7 +1286,7 @@ module M = {
         s_r4r4x5, s_r2r2, s_r2r2x5);
         leakages <- LeakExpr([]) :: leakages;
         b64 <- s_b64;
-      leakages <- LeakCond(((W64.of_uint 0) `<` b64)) :: LeakExpr([]) :: leakages;
+      leakages <- LeakCond(((W64.of_uint 0) \ult b64)) :: LeakExpr([]) :: leakages;
       
       }
       leakages <- LeakExpr([]) :: leakages;
@@ -1350,9 +1301,9 @@ module M = {
     leakages <- LeakExpr([]) :: leakages;
     b16 <- (b16 `&` (W64.of_uint 3));
     
-    leakages <- LeakCond(((W64.of_uint 0) `<` b16)) :: LeakExpr([]) :: leakages;
+    leakages <- LeakCond(((W64.of_uint 0) \ult b16)) :: LeakExpr([]) :: leakages;
     
-    while (((W64.of_uint 0) `<` b16)) {
+    while (((W64.of_uint 0) \ult b16)) {
       leakages <- LeakExpr([]) :: leakages;
       b16 <- (b16 - (W64.of_uint 1));
       leakages <- LeakExpr([]) :: leakages;
@@ -1365,7 +1316,7 @@ module M = {
       h <@ mulmod_12 (h, s_r, s_rx5);
       leakages <- LeakExpr([]) :: leakages;
       h <@ carry_reduce (h);
-    leakages <- LeakCond(((W64.of_uint 0) `<` b16)) :: LeakExpr([]) :: leakages;
+    leakages <- LeakCond(((W64.of_uint 0) \ult b16)) :: LeakExpr([]) :: leakages;
     
     }
     leakages <- LeakExpr([]) :: leakages;
